src/frontends/lean/info_manager.h
@@ -11,8 +11,7 @@ Author: Leonardo de Moura
 #include "kernel/expr.h"
 #include "library/io_state_stream.h"
 #include "library/metavar_context.h"
-#include "library/tactic/tactic_state.h"
-#include "library/tactic/smt/smt_state.h"
+#include "library/vm/vm.h"
 #include "frontends/lean/json.h"
 
 namespace lean {
@@ -43,28 +42,6 @@ public:
     vm_obj_format_info(environment const & env, vm_obj const & thunk):m_env(env), m_thunk(thunk) {}
 #ifdef LEAN_JSON
     virtual void report(io_state_stream const & ios, json & record) const;
-#endif
-};
-
-class tactic_state_info_data : public info_data_cell {
-protected:
-    tactic_state m_state;
-public:
-    tactic_state_info_data(tactic_state const & s):m_state(s) {}
-
-#ifdef LEAN_JSON
-    virtual void report(io_state_stream const &, json & record) const override;
-#endif
-};
-
-class smt_tactic_state_info_data : public tactic_state_info_data {
-    list<smt_goal> m_smt_state;
-public:
-    smt_tactic_state_info_data(list<smt_goal> const & ss, tactic_state const & ts):
-        tactic_state_info_data(ts), m_smt_state(ss) {}
-
-#ifdef LEAN_JSON
-    virtual void report(io_state_stream const &, json & record) const override;
 #endif
 };
 
@@ -108,8 +85,6 @@ public:
 
     void add_type_info(unsigned l, unsigned c, expr const & e);
     void add_identifier_info(unsigned l, unsigned c, name const & full_id);
-    void add_tactic_state_info(unsigned l, unsigned c, tactic_state const & s);
-    void add_smt_tactic_state_info(unsigned l, unsigned c, list<smt_goal> const & ss, tactic_state const & ts);
     void add_vm_obj_format_info(unsigned l, unsigned c, environment const & env, vm_obj const & thunk);
 
     void instantiate_mvars(metavar_context const & mctx);
