src/frontends/lean/tactic_evaluator.cpp
@@ -63,28 +63,6 @@ vm_obj tactic_evaluator::invoke_tactic(vm_state & S, name const & tactic_name, s
     return r;
 }
 
-void tactic_evaluator::add_tactic_state_info(tactic_state const & s, expr const & ref) {
-    if (!get_global_info_manager()) return;
-    pos_info_provider * pip = get_pos_info_provider();
-    if (!pip) return;
-    if (auto p = pip->get_pos_info(ref))
-        m_info.add_tactic_state_info(p->first, p->second, s);
-}
-
-static list<smt_goal> to_smt_state(vm_obj const & ss) {
-    return to_list<smt_goal>(ss, to_smt_goal);
-}
-
-void tactic_evaluator::add_smt_tactic_state_info(vm_obj const & ss, tactic_state const & ts, expr const & ref) {
-    if (!get_global_info_manager()) return;
-    pos_info_provider * pip = get_pos_info_provider();
-    if (!pip) return;
-    if (auto p = pip->get_pos_info(ref)) {
-        list<smt_goal> _ss = to_smt_state(ss);
-        m_info.add_smt_tactic_state_info(p->first, p->second, _ss, ts);
-    }
-}
-
 static void process_failure(vm_state & S, vm_obj const & r, expr const & ref) {
     pos_info_provider * provider = get_pos_info_provider();
     if (optional<tactic_exception_info> ex = is_tactic_exception(S, r)) {
@@ -99,12 +77,8 @@ static void process_failure(vm_state & S, vm_obj const & r, expr const & ref) {
 }
 
 tactic_state tactic_evaluator::execute_tactic(expr const & tactic, tactic_state const & s, expr const & ref) {
-    pos_info_provider * provider = get_pos_info_provider();
-    scope_traces_as_messages traces_as_messages(provider, ref);
-
     name tactic_name("_tactic");
     environment new_env = compile_tactic(tactic_name, tactic);
-
     vm_state S(new_env, m_opts);
     vm_obj r = invoke_tactic(S, tactic_name, {to_obj(s)});
 
@@ -115,148 +89,15 @@ tactic_state tactic_evaluator::execute_tactic(expr const & tactic, tactic_state 
     lean_unreachable();
 }
 
-pair<vm_obj, tactic_state> tactic_evaluator::execute_smt_tactic(expr const & tactic, vm_obj const & ss, tactic_state const & ts, expr const & ref) {
-    pos_info_provider * provider = get_pos_info_provider();
-    scope_traces_as_messages traces_as_messages(provider, ref);
-
-    name tactic_name("_smt_tactic");
-    environment new_env = compile_tactic(tactic_name, tactic);
-
-    vm_state S(new_env, m_opts);
-    vm_obj r = invoke_tactic(S, tactic_name, {to_obj(ts), ss});
-
-    if (is_tactic_result_success(r)) {
-        vm_obj new_ss       = cfield(get_tactic_result_value(r), 1);
-        tactic_state new_ts = to_tactic_state(get_tactic_result_state(r));
-        return mk_pair(new_ss, new_ts);
-    }
-    process_failure(S, r, ref);
-    lean_unreachable();
-}
-
-bool is_smt_begin_end_block(expr const & tactic) {
-    return
-        is_app_of(tactic, get_smt_tactic_execute_name(), 1) ||
-        is_app_of(tactic, get_smt_tactic_execute_with_name(), 2);
-}
-
-tactic_state tactic_evaluator::execute_begin_end(tactic_state const & s, buffer<expr> const & tactics, expr const & ref) {
-    lean_assert(!tactics.empty());
-    list<expr> gs = s.goals();
-    if (!gs) throw elaborator_exception(ref, "tactic failed, there are no goals to be solved");
-    tactic_state new_s = set_goals(s, to_list(head(gs)));
-    for (expr const & tactic : tactics) {
-        expr const & curr_ref = tactic;
-        if (is_begin_end_element(tactic)) {
-            add_tactic_state_info(new_s, curr_ref);
-            new_s = execute_tactic(get_annotation_arg(tactic), new_s, curr_ref);
-        } else if (is_begin_end_block(tactic)) {
-            buffer<expr> nested_tactics;
-            get_begin_end_block_elements(tactic, nested_tactics);
-            new_s = execute_begin_end(new_s, nested_tactics, curr_ref);
-        } else if (is_smt_begin_end_block(tactic)) {
-            new_s = execute_smt_begin_end(new_s, tactic, curr_ref);
-        } else {
-            throw elaborator_exception(curr_ref, "ill-formed 'begin ... end' tactic block");
-        }
-    }
-    add_tactic_state_info(new_s, ref);
-    if (new_s.goals()) throw_unsolved_tactic_state(new_s, "tactic failed, there are unsolved goals", ref);
-    return set_goals(new_s, tail(gs));
-}
-
 tactic_state tactic_evaluator::execute_atomic(tactic_state const & s, expr const & tactic, expr const & ref) {
-    add_tactic_state_info(s, ref);
-    /* Save information using tactic's position, ref is usually the `by` token position */
-    add_tactic_state_info(s, tactic);
     tactic_state new_s = execute_tactic(tactic, s, ref);
     if (new_s.goals())
         throw_unsolved_tactic_state(new_s, "tactic failed, there are unsolved goals", ref);
     return new_s;
 }
 
-pair<vm_obj, tactic_state> tactic_evaluator::mk_smt_state(tactic_state const & s, expr const & smt_cfg, expr const & ref) {
-    /*
-      smt_state.mk              : smt_config → tactic smt_state
-    */
-    expr value = mk_app(mk_constant(get_smt_state_mk_name()), smt_cfg);
-    expr type  = m_ctx.infer(value);
-    environment new_env  = m_ctx.env();
-    bool use_conv_opt    = true;
-    bool is_trusted      = false;
-    name init_state_name("_init_state");
-    auto cd = check(new_env, mk_definition(new_env, init_state_name, {}, type, value, use_conv_opt, is_trusted));
-    new_env = new_env.add(cd);
-    try {
-        new_env = vm_compile(new_env, new_env.get(init_state_name));
-    } catch (exception & ex) {
-        throw elaborator_exception(ref, ex.what());
-    }
-    vm_state S(new_env, m_opts);
-    vm_obj r = S.invoke(init_state_name, to_obj(s));
-    if (is_tactic_result_success(r)) {
-        return mk_pair(get_tactic_result_value(r), to_tactic_state(get_tactic_result_state(r)));
-    }
-    tactic_exception_info info = *is_tactic_exception(S, r);
-    throw elaborator_exception(ref,
-                               format("failed to execute smt_tactic, initial smt_state could not be constructed, nested error:") +
-                               line() + std::get<0>(info));
-}
-
-pair<vm_obj, tactic_state> tactic_evaluator::execute_smt_begin_end_core(vm_obj const & ss, tactic_state const & ts, buffer<expr> const & tactics, expr const & ref) {
-    lean_assert(!tactics.empty());
-    list<expr> gs = ts.goals();
-    if (!gs) throw elaborator_exception(ref, "smt_tactic failed, there are no goals to be solved");
-    if (is_nil(ss)) throw elaborator_exception(ref, "smt_tactic failed, there are no smt goals to be solved");
-
-    tactic_state new_ts = set_goals(ts, to_list(head(gs)));
-    vm_obj new_ss       = mk_vm_cons(head(ss), mk_vm_nil());
-
-    for (expr const & tactic : tactics) {
-        expr const & curr_ref = tactic;
-        if (is_begin_end_element(tactic)) {
-            add_smt_tactic_state_info(new_ss, new_ts, curr_ref);
-            std::tie(new_ss, new_ts) = execute_smt_tactic(get_annotation_arg(tactic), new_ss, new_ts, curr_ref);
-        } else if (is_begin_end_block(tactic)) {
-            buffer<expr> nested_tactics;
-            get_begin_end_block_elements(tactic, nested_tactics);
-            std::tie(new_ss, new_ts) = execute_smt_begin_end_core(new_ss, new_ts, nested_tactics, curr_ref);
-        } else {
-            throw elaborator_exception(curr_ref, "ill-formed 'begin ... end' smt_tactic block");
-        }
-    }
-    add_smt_tactic_state_info(new_ss, new_ts, ref);
-    if (new_ts.goals()) throw_unsolved_smt_tactic_state(new_ss, new_ts, "tactic failed, there are unsolved goals", ref);
-    new_ts = set_goals(new_ts, tail(gs));
-    new_ss = tail(ss);
-    return mk_pair(new_ss, new_ts);
-}
-
-tactic_state tactic_evaluator::execute_smt_begin_end(tactic_state ts, expr tactic, expr const & ref) {
-    lean_assert(is_smt_begin_end_block(tactic));
-    expr smt_cfg;
-    if (is_app_of(tactic, get_smt_tactic_execute_with_name(), 2))
-        smt_cfg = app_arg(app_fn(tactic));
-    else
-        smt_cfg = copy_tag(ref, mk_constant(get_default_smt_config_name()));
-    tactic = app_arg(tactic);
-    buffer<expr> tactics;
-    get_begin_end_block_elements(tactic, tactics);
-    vm_obj ss;
-    std::tie(ss, ts) = mk_smt_state(ts, smt_cfg, ref);
-    return execute_smt_begin_end_core(ss, ts, tactics, ref).second;
-}
-
 tactic_state tactic_evaluator::operator()(tactic_state const & s, expr const & tactic, expr const & ref) {
-    if (is_begin_end_block(tactic)) {
-        buffer<expr> tactics;
-        get_begin_end_block_elements(tactic, tactics);
-        return execute_begin_end(s, tactics, ref);
-    } else if (is_smt_begin_end_block(tactic)) {
-        return execute_smt_begin_end(s, tactic, ref);
-    } else {
-        return execute_atomic(s, tactic, ref);
-    }
+    return execute_atomic(s, tactic, ref);
 }
 
 tactic_evaluator::tactic_evaluator(type_context & ctx, info_manager & info, options const & opts):
