src/frontends/lean/tactic_notation.h
@@ -12,10 +12,6 @@ expr parse_curly_begin_end_expr(parser & p, pos_info const & pos);
 expr parse_begin_end(parser & p, unsigned, expr const *, pos_info const & pos);
 expr parse_by(parser & p, unsigned, expr const *, pos_info const & pos);
 expr parse_auto_quote_tactic_block(parser & p, unsigned, expr const *, pos_info const & pos);
-bool is_begin_end_block(expr const & e);
-bool is_begin_end_element(expr const & e);
-void get_begin_end_block_elements(expr const & e, buffer<expr> & elems);
-expr update_begin_end_block(expr const & e, buffer<expr> const & elems);
 void initialize_tactic_notation();
 void finalize_tactic_notation();
 }
