library/init/util.lean
@@ -5,15 +5,21 @@ Authors: Leonardo de Moura
 -/
 prelude
 import init.data.string.basic
+universe variables u
 
 /- This function has a native implementation that tracks time. -/
-def timeit {α : Type} (s : string) (f : unit → α) : α :=
+def timeit {α : Type u} (s : string) (f : unit → α) : α :=
 f ()
 
 /- This function has a native implementation that displays the given string in the regular output stream. -/
-def trace {α : Type} (s : string) (f : unit → α) : α :=
+def trace {α : Type u} (s : string) (f : unit → α) : α :=
 f ()
 
 /- This function has a native implementation that shows the VM call stack. -/
-def trace_call_stack {α : Type} (f : unit → α) : α :=
+def trace_call_stack {α : Type u} (f : unit → α) : α :=
+f ()
+
+/- This function has a native implementation that displays in the given position all trace messages used in f.
+   The arguments line and col are filled by the elaborator. -/
+def scope_trace {α : Type u} {line col: nat} (f : unit → α) : α :=
 f ()
