library/init/meta/tactic.lean
@@ -408,6 +408,7 @@ try $ do
 /- (save_type_info e ref) save (typeof e) at position associated with ref -/
 meta constant save_type_info : expr → expr → tactic unit
 meta constant save_info_thunk : nat → nat → (unit → format) → tactic unit
+meta constant report_error : nat → nat → format → tactic unit
 /- Return list of currently opened namespace -/
 meta constant open_namespaces : tactic (list name)
 open list nat
@@ -419,6 +420,15 @@ get_goals >>= set_goals
 /- Auxiliary definition used to implement begin ... end blocks -/
 meta def step {α : Type u} (t : tactic α) : tactic unit :=
 t >>[tactic] cleanup
+
+/- Auxiliary definition used to implement begin ... end blocks.
+   It is similar to step, but it reports an error at the given line/col if the tactic t fails. -/
+meta def rstep {α : Type u} (line : nat) (col : nat) (t : tactic α) : tactic unit :=
+λ s, tactic_result.cases_on (@scope_trace _ line col (λ _, (t >>[tactic] cleanup) s))
+  (λ a new_s, tactic_result.success () new_s)
+  (λ msg_thunk e new_s,
+    let msg := msg_thunk () ++ format.line ++ to_fmt "state:" ++ format.line ++ new_s^.to_format in
+        (tactic.report_error line col msg >> tactic.failed) new_s)
 
 meta def is_prop (e : expr) : tactic bool :=
 do t ← infer_type e,
@@ -556,6 +566,10 @@ do { ctx ← local_context,
      H   ← find_same_type t ctx,
      exact H }
 <|> fail "assumption tactic failed"
+
+meta def save_info (line : nat) (col : nat) : tactic unit :=
+do s ← read,
+   tactic.save_info_thunk line col (λ _, tactic_state.to_format s)
 
 notation `‹` p `›` := show p, by assumption
 
