tests/lean/run/my_tac_class.lean
@@ -1,0 +1,63 @@
+meta def mytac :=
+state_t nat tactic
+
+meta instance : monad mytac :=
+state_t.monad _ _
+
+meta instance : monad.has_monad_lift tactic mytac :=
+monad.monad_transformer_lift (state_t nat) tactic
+
+meta instance (α : Type) : has_coe (tactic α) (mytac α) :=
+⟨monad.monad_lift⟩
+
+namespace mytac
+
+meta def step {α : Type} (t : mytac α) : mytac unit :=
+t >> return ()
+
+meta def rstep {α : Type} (line : nat) (col : nat) (t : mytac α) : mytac unit :=
+λ v s, tactic_result.cases_on (@scope_trace _ line col (λ _, t v s))
+  (λ ⟨a, v⟩ new_s, tactic_result.success ((), v) new_s)
+  (λ msg_thunk e new_s,
+    let msg := msg_thunk () ++ format.line ++ to_fmt "value: " ++ to_fmt v ++ format.line ++ to_fmt "state:" ++ format.line ++ new_s^.to_format in
+        (tactic.report_error line col msg >> tactic.failed) new_s)
+
+meta def execute (tac : mytac unit) : tactic unit :=
+tac 0 >> return ()
+
+meta def save_info (line col : nat) : mytac unit :=
+do v ← state_t.read,
+   s ← tactic.read,
+   tactic.save_info_thunk line col
+      (λ _, to_fmt "Custom state: " ++ to_fmt v ++ format.line ++
+                tactic_state.to_format s)
+
+namespace interactive
+meta def intros : mytac unit :=
+tactic.intros >> return ()
+
+meta def constructor : mytac unit :=
+tactic.constructor
+
+meta def trace (s : string) : mytac unit :=
+tactic.trace s
+
+meta def assumption : mytac unit :=
+tactic.assumption
+
+meta def inc : mytac unit :=
+do v ← state_t.read, state_t.write (v+1)
+
+end interactive
+end mytac
+
+example (p q : Prop) : p → q → p ∧ q :=
+begin [mytac]
+  intros,
+  inc,
+  trace "test",
+  constructor,
+  inc,
+  assumption,
+  assumption
+end
